-

Examples/Remdups.thy
@@ -2,7 +2,7 @@ theory Remdups
   imports "../Refine_Imperative_HOL/Sepref" "SepLogicTime_RBTreeBasic.RBTree_Impl"
     "../Refine_Imperative_HOL/IICF/Impl/IICF_Rbt_Set"  
     "../Refine_Imperative_HOL/IICF/Impl/IICF_DArray_List"  
- "../RefineMonadicVCG"
+ "../RefineMonadicVCG" "../Refine_Foreach"
 begin
         
 
@@ -35,7 +35,7 @@ definition rd_impl1 :: "('a::{heap,linorder}) list \<Rightarrow> ('a list) nrest
   }) (zs,ys,S);
   RETURNT ys
   }"
-
+ 
 definition "remdups_time (n::nat) = n * body_time n + 20"
 
 definition "remdups_spec as = REST (emb (\<lambda>ys. set as = set ys \<and> distinct ys)
@@ -55,7 +55,50 @@ lemma rd_impl1_correct: "rd_impl1 as \<le> remdups_spec as"
         apply (auto simp:
               Some_le_mm3_Some_conv
           body_time_def remdups_time_def)
+    done
+ 
+(*
+definition rd_impl2 :: "('a::{heap,linorder}) list \<Rightarrow> ('a list) nrest" where
+"rd_impl2 as = do {
+  ys \<leftarrow> mop_empty_list 12;
+  S \<leftarrow> mop_set_empty 1;
+  zs \<leftarrow> RETURNT as;
+  nfoldli as (\<lambda>_. True) (\<lambda>x (ys,S). do {    
+    ASSERT (length ys \<le> length as);
+    ASSERT (card S \<le> length ys);
+    b \<leftarrow> mop_set_member (\<lambda>S. rbt_search_time_logN (length as + 1) + 1) x S;
+    if b then
+      RETURNT (ys,S)
+    else do {
+      S \<leftarrow> mop_set_insert (\<lambda>S. rbt_insert_logN (length as + 1)) x S;
+      ys \<leftarrow> mop_push_list (\<lambda>_. 23) x ys;  
+      RETURNT (ys,S)
+    } 
+  }) (ys,S);
+  RETURNT ys
+  }"
+
+
+
+lemma rd_impl2_correct: "rd_impl2 as \<le> remdups_spec as"
+  unfolding remdups_spec_def
+  unfolding rd_impl2_def mop_empty_list_def mop_set_empty_def mop_set_member_def mop_set_insert_def mop_push_list_def
+      rd_ta_def rd_inv_def
+  apply(rule T_specifies_I)
+  apply (vcg' \<open>simp\<close> )
+  unfolding nfoldliIE_def[where E="2*rbt_search_time_logN (length as + 1) + 24"
+                            and I="\<lambda>l1 l2 (bs,S). set l1 = S \<and> set bs = S \<and> distinct bs", symmetric] 
+  apply(rule nfoldliIE_rule[  THEN T_specifies_rev, THEN T_conseq4]) 
+  apply (vcg' \<open>simp\<close> rules: nfoldliIE_rule[  THEN T_specifies_rev, THEN T_conseq4])
+  apply(rule T_specifies_I)
+      apply (vcg' \<open>simp\<close>) 
+    unfolding Some_le_emb'_conv Some_eq_emb'_conv 
+  supply [simp] = neq_Nil_conv distinct_length_le card_length
+        apply (a uto simp:
+              Some_le_mm3_Some_conv
+          body_time_def remdups_time_def)
   done
+*)
  
 lemma remdups_time_nln[asym_bound]: "remdups_time \<in> \<Theta>(\<lambda>n. n * ln n)"
   unfolding remdups_time_def body_time_def
@@ -108,7 +151,7 @@ declare rbt_search_time_logN_mono [intro]
 declare rbt_insert_logN_mono [intro]
 
 sepref_definition remdups_impl is "uncurry0 (rd_impl1 as)" :: "unit_assn\<^sup>k \<rightarrow>\<^sub>a da_assn id_assn"
-  unfolding rd_impl1_def whileIET_def 
+  unfolding rd_impl1_def whileIET_def    
   apply sepref_dbg_keep 
   done
 print_theorems
